LambdaS5/coq/EjsToLjs.v
@@ -130,7 +130,7 @@ Definition new_context_in ctx e :=
 
 Definition derived_context_in flds e :=
     let objattrs := L.objattrs_intro (L.expr_string "DeclEnvRec") 
-        L.expr_true L.expr_null L.expr_undefined L.expr_null in
+        L.expr_true L.expr_null L.expr_undefined in
     new_context_in (L.expr_object objattrs [("parent", L.expr_id "$parent")] flds) e.
 
 Definition make_var_decl is e := 
@@ -250,7 +250,7 @@ Definition make_array es :=
     let mkprop e := L.property_data (L.data_intro e L.expr_true L.expr_true L.expr_true) in
     let exp_props := number_list_from 0 (map mkprop es) in
     let l_prop := L.property_data (L.data_intro (L.expr_number (length exp_props)) L.expr_true L.expr_false L.expr_false) in
-    let attrs := L.objattrs_intro (L.expr_string "Array") L.expr_true (make_builtin "%ArrayProto") L.expr_null L.expr_undefined in 
+    let attrs := L.objattrs_intro (L.expr_string "Array") L.expr_true (make_builtin "%ArrayProto") L.expr_null in 
     L.expr_object attrs nil (("length", l_prop) :: exp_props).
 
 Definition make_args_obj (es : list L.expr) := 
@@ -313,7 +313,7 @@ Definition combine_props ps :=
 Definition make_object ps :=    
     let gs_ids := remove_dupes (map fst ps) in
     let props := map (fun s => (s, combine_props (assocs s ps))) gs_ids in
-    let oa := L.objattrs_intro (L.expr_string "Object") L.expr_true (make_builtin "%ObjectProto") L.expr_undefined L.expr_undefined in
+    let oa := L.objattrs_intro (L.expr_string "Object") L.expr_true (make_builtin "%ObjectProto") L.expr_undefined in
     L.expr_object oa nil props.
 
 Definition make_new e es := make_app_builtin "%PrimNew" [e; make_args_obj es].
